theories/typing/lib/ghostptrtoken/ghostptrtoken.v
@@ -1,0 +1,229 @@
+From lrust.typing Require Export type.
+From lrust.typing Require Import array_util typing.
+Set Default Proof Using "Type".
+
+Open Scope nat.
+Implicit Type 𝔄 𝔅: syn_type.
+
+Section token.
+  Context `{!typeG Σ}.
+
+  Lemma split_mt_token {𝔄} d l' amπ Φ :
+    (l' ↦∗: (λ vl, [S(d') := d] ∃ (aπm: gmap loc (proph 𝔄)),
+      ⌜vl = [] ∧ amπ = mapply aπm⌝ ∗ Φ d' aπm)) ⊣⊢
+    [S(d') := d] ∃(aπm: gmap loc (proph 𝔄)),
+      ⌜amπ = mapply aπm⌝ ∗ l' ↦∗ [] ∗ Φ d' aπm.
+  Proof.
+    iSplit.
+    - iIntros "(%& ↦ & big)". case d=>// ?. iDestruct "big" as (?[->->]) "Φ".
+      iExists _. iSplit; [done|iFrame].
+    - iIntros "big". case d=>// ?. iDestruct "big" as (?->) "(↦ & ?)".
+      iExists []. iFrame "↦". iExists _. by iFrame.
+  Qed.
+
+  Lemma split_mt_token' {𝔄} l' amπ Φ :
+    (l' ↦∗: (λ vl, ∃(aπm: gmap loc (proph 𝔄)),
+      ⌜vl = [] ∧ amπ = mapply aπm⌝ ∗ Φ aπm)) ⊣⊢
+    ∃(aπm: gmap loc (proph 𝔄)),
+      ⌜amπ = mapply aπm⌝ ∗ l' ↦∗ [] ∗ Φ aπm.
+  Proof.
+    set Φ' := λ _: nat, Φ. have ->: Φ = Φ' 0 by done.
+    by apply (split_mt_token (S _)).
+  Qed.
+
+  Lemma ty_share_big_sepM {𝔄} (ty: type 𝔄) E aπm d κ tid q :
+    ↑lftN ⊆ E → lft_ctx -∗ κ ⊑ ty_lft ty -∗
+    &{κ} ([∗ map] l ↦ aπ ∈ aπm, l ↦∗: ty.(ty_own) aπ d tid) -∗ q.[κ]
+      ={E}=∗ |={E}▷=>^d |={E}=>
+        ([∗ map] l ↦ aπ ∈ aπm, ty.(ty_shr) aπ d κ tid l) ∗ q.[κ].
+  Proof.
+    rewrite big_opM_map_to_list.
+    rewrite big_opM_map_to_list.
+    iIntros (?) "#LFT #In Bor κ".
+    iMod (bor_big_sepL with "LFT Bor") as "Bors"; [done|].
+    iInduction (map_to_list aπm) as [|] "IH" forall (q)=>/=.
+    { iApply step_fupdN_full_intro. by iFrame. }
+    iDestruct "κ" as "[κ κ₊]". iDestruct "Bors" as "[Bor Bors]".
+    iMod (ty_share with "LFT In Bor κ") as "Toshr"; [done|].
+    iMod ("IH" with "κ₊ Bors") as "Toshrs".
+    iCombine "Toshr Toshrs" as "Toshrs". iApply (step_fupdN_wand with "Toshrs").
+    by iIntros "!> [>[$$] >[$$]]".
+  Qed.
+
+  Lemma trans_big_sepM_mt_ty_own {𝔄} (ty: type 𝔄) aπm d tid :
+    ([∗ list] elt ∈ aπm, elt.1 ↦∗: ty.(ty_own) elt.2 d tid) ⊣⊢
+    ∃(wll: vec (list val) (length aπm)), ([∗ list] elt ∈ (vzip (vmap (λ x, x.1) (Vector.of_list aπm)) wll), elt.1 ↦∗ elt.2) ∗
+      ([∗ list] aπwl ∈ vzip (vmap (λ x, x.2) (Vector.of_list aπm)) wll, ty.(ty_own) aπwl.1 d tid aπwl.2).
+  Proof.
+    iSplit.
+    - iIntros "↦owns". iInduction aπm as [|] "IH"=>/=.
+      { iExists [#]. iSplit; [done|done]. }
+      iDestruct "↦owns" as "[(%& ↦ & ty) ↦owns]".
+      iDestruct ("IH" with "↦owns") as (?) "(↦s & tys)".
+      iExists (_:::_). iFrame.
+    - iIntros "(%& ↦s & tys)". iInduction aπm as [|] "IH"; [done|].
+      inv_vec wll=>/= ??.
+      iDestruct "↦s" as "[↦ ↦s]". iDestruct "tys" as "[ty tys]".
+      iSplitL "↦ ty".
+      { iExists _. iFrame. }
+      iApply ("IH" with "↦s tys").
+  Qed.
+
+  Definition list_to_gmap {A} `{Countable K} : list (K * A) → gmap K A := list_to_map.
+
+  Lemma remove_mapply {A B} `{Countable K} π (aπm: gmap K (A → B)):
+    mapply aπm π = list_to_map (prod_map id (.$ π) <$> (map_to_list aπm)).
+  Proof.
+    rewrite list_to_map_fmap. rewrite list_to_map_to_list. exact.
+  Qed.
+
+  Lemma remove_mapply2 {𝔄} `{Countable K} ξl (aπm: gmap K (proph 𝔄)):
+    (mapply aπm ./ ξl) <-> (λ π, list_to_gmap (prod_map id (.$ π) <$> (map_to_list aπm))) ./ ξl.
+  Proof.
+    split.
+    intros. intros π π' eqv. specialize (H0 π π' eqv).
+    rewrite 2! remove_mapply in H0. exact.
+    intros. intros π π' eqv. specialize (H0 π π' eqv).
+    rewrite 2! remove_mapply. exact.
+  Qed.
+
+  Lemma ty_own_proph_big_sepM_mt {𝔄} (ty: type 𝔄) (n: nat) E aπm d tid κ q :
+  ↑lftN ⊆ E → lft_ctx -∗ κ ⊑ ty_lft ty -∗
+  ([∗ map] l ↦ aπ ∈ aπm, l ↦∗: ty.(ty_own) aπ d tid) -∗ q.[κ]
+    ={E}=∗ |={E}▷=>^d |={E}=> ∃ξl q', ⌜mapply aπm ./ ξl⌝ ∗ q':+[ξl] ∗
+      (q':+[ξl] ={E}=∗
+        ([∗ map] l ↦ aπ ∈ aπm, l ↦∗: ty.(ty_own) aπ d tid) ∗ q.[κ]).
+  Proof.
+    rewrite {1} big_opM_map_to_list.
+    rewrite {1} trans_big_sepM_mt_ty_own. iIntros (?) "LFT In (%& ↦ & tys) κ".
+    iMod (ty_own_proph_big_sepL with "LFT In tys κ") as "Upd"; [done|].
+    iApply (step_fupdN_wand with "Upd"). iIntros "!> >(%&%&%& ξl & Totys) !>".
+    iExists _, _.
+    apply proph_dep_constr with vec_to_list _ _  in H0. rewrite vec_to_list_apply in H0.
+    rewrite vec_to_list_map in H0. rewrite vec_to_list_to_vec in H0.
+    apply proph_dep_constr with (λ x, zip ((map_to_list aπm).*1) x) _ _  in H0.
+    iSplit. iPureIntro.
+    rewrite remove_mapply2.
+    apply proph_dep_constr.
+    unfold compose in H0. unfold lapply in H0.
+    intros π π' eqv. specialize (H0 π π' eqv).
+    rewrite zip_with_fmap_r in H0. rewrite zip_with_fst_snd in H0.
+    rewrite zip_with_fmap_r in H0. rewrite zip_with_fst_snd in H0.
+    assert (forall π,(uncurry (λ (x: loc) (z: (proph (of_syn_type 𝔄))) , (x, z π))) = prod_map id (.$ π)).
+    intros. apply functional_extensionality. intros. destruct x.
+    unfold prod_map. unfold uncurry. unfold Datatypes.uncurry. unfold fst. unfold snd. unfold id. reflexivity.
+    rewrite 2! H1 in H0. exact H0.
+    iIntros "{$ξl}ξl".
+    iMod ("Totys" with "ξl") as "[tys $]".
+    rewrite big_opM_map_to_list. rewrite trans_big_sepM_mt_ty_own.
+    iModIntro. iExists _. iFrame.
+  Qed.
+
+  Lemma ty_shr_proph_big_sepM {𝔄} (ty: type 𝔄) (n: nat) E aπm d κ tid κ' q :
+  ↑lftN ⊆ E → lft_ctx -∗ κ' ⊑ κ -∗ κ' ⊑ ty_lft ty -∗
+  ([∗ map] l ↦ aπ ∈ aπm, ty.(ty_shr) aπ d κ tid l) -∗ q.[κ']
+    ={E}▷=∗ |={E}▷=>^d |={E}=> ∃ξl q', ⌜mapply aπm ./ ξl⌝ ∗ q':+[ξl] ∗
+      (q':+[ξl] ={E}=∗ q.[κ']).
+  Proof.
+    iIntros (?) "#LFT #In #In' tys κ'".
+    rewrite big_opM_map_to_list.
+    setoid_rewrite remove_mapply2.
+    iInduction (map_to_list aπm) as [|] "IH" forall (q).
+    { iApply step_fupdN_full_intro. iIntros "!>!>!>!>". iExists [], 1%Qp.
+      iFrame "κ'". iSplit.
+      iPureIntro. intros π π' eqv. rewrite 2! fmap_nil. reflexivity.
+      iSplit; [done|].
+      by iIntros. }
+    iDestruct "κ'" as "[κ' κ'₊]". iDestruct "tys" as "[ty tys]".
+    iMod (ty_shr_proph with "LFT In In' ty κ'") as "Upd"; [done|].
+    iMod ("IH" with "tys κ'₊") as "Upd'".
+    iIntros "!>!>". iCombine "Upd Upd'" as "Upd". iApply (step_fupdN_wand with "Upd").
+    iIntros "[>(%&%&%& ξl & Toκ') >(%&%&%& ζl & Toκ'₊)] !>".
+    iDestruct (proph_tok_combine with "ξl ζl") as (?) "[ξζl Toξζl]".
+    iExists _, _. iFrame "ξζl". iSplit.
+    iPureIntro. intros π π' eqv. 
+    rewrite 2! fmap_cons. unfold list_to_gmap. unfold list_to_gmap in H1.
+    rewrite 2! list_to_map_cons. congr insert. 
+    apply H0. intros ξ ξin. apply eqv. apply elem_of_app. left. exact.
+    apply H1. intros ξ ξin. apply eqv. apply elem_of_app. right. exact.  
+    iIntros "ξζl". iDestruct ("Toξζl" with "ξζl") as "[ξl ζl]".
+    iMod ("Toκ'" with "ξl") as "$". by iMod ("Toκ'₊" with "ζl") as "$".
+  Qed.
+
+  (* Rust's GhostPtrToken<T> *)
+  Program Definition ghostptrtoken_ty {𝔄} (ty: type 𝔄) : type (fmapₛ 𝔄) := {|
+    ty_size := 0;  ty_lfts := ty.(ty_lfts);  ty_E := ty.(ty_E);
+    ty_own amπ d tid vl :=
+      [S(d') := d] ∃(aπm: gmap loc (proph 𝔄)),
+        ⌜vl = [] ∧ amπ = mapply aπm⌝ ∗
+        ▷ ([∗ map] l ↦ aπ ∈ aπm, (l) ↦∗: ty.(ty_own) aπ d' tid) ∗
+        ([∗ map] l ↦ _ ∈ aπm, freeable_sz' ty.(ty_size) l);
+    ty_shr amπ d κ tid l' :=
+      [S(d') := d] ∃(aπm: gmap loc (proph 𝔄)),
+        ⌜amπ = mapply aπm⌝ ∗
+        ▷ [∗ map] l ↦ aπ ∈ aπm, ty.(ty_shr) aπ d' κ tid l;
+  |}%I.
+  Next Obligation.
+    iIntros (???[]??) "token //". by iDestruct "token" as (?[-> _]) "?".
+  Qed.
+  Next Obligation.
+    move=> ??[|?][|?]*/=; try (by iIntros); [lia|]. do 11 f_equiv.
+    apply ty_own_depth_mono. lia.
+  Qed.
+  Next Obligation.
+    move=> ??[|?][|?]*/=; try (by iIntros); [lia|]. do 7 f_equiv.
+    apply ty_shr_depth_mono. lia.
+  Qed.
+  Next Obligation.
+    move=> ?????[|?]*; [by iIntros|]. iIntros "#? (%&?& All)".
+    iExists _. iSplit; [done|].
+    rewrite !big_sepM_forall. iIntros "!> **".
+    iApply ty_shr_lft_mono; by [|iApply "All"].
+  Qed.
+  Next Obligation.
+    iIntros (???? d) "*% #LFT In Bor κ". rewrite split_mt_token. case d.
+    { by iMod (bor_persistent with "LFT Bor κ") as "[>[] _]". }
+    move=> ?. do 1 (iMod (bor_exists_tok with "LFT Bor κ") as (?) "[Bor κ]"; [done|]).
+    iMod (bor_sep_persistent with "LFT Bor κ") as "(>-> & Bor & κ)"; [done|].
+    iMod (bor_sep with "LFT Bor") as "[Bor↦ Bor]"; [done|].
+    iMod (bor_fracture (λ q', _ ↦∗{q'} _)%I with "LFT Bor↦") as "Bor↦"; [done|].
+    iMod (bor_sep with "LFT Bor") as "[Bor _]"; [done|].
+    iMod (bor_later_tok with "LFT Bor κ") as "Borκ"; [done|].
+    iIntros "/=!>!>!>". iMod "Borκ" as "[Bor κ]".
+    iMod (ty_share_big_sepM with "LFT In Bor κ") as "Toshrs"; [done|].
+    iApply (step_fupdN_wand with "Toshrs"). iIntros "!> >[?$] !>".
+    iExists _. by iFrame.
+  Qed.
+  Next Obligation.
+    iIntros (????[|?]) "*% LFT In token κ/="; [done|].
+    iDestruct "token" as (?[->->]) "(↦tys & †)". iIntros "!>!>!>".
+    iMod (ty_own_proph_big_sepM_mt with "LFT In ↦tys κ") as "Upd"; [done|done|].
+    iApply (step_fupdN_wand with "Upd"). iIntros "!> >(%&%&%& ξl & Totys) !>".
+    iExists _, _. iSplit; [done|].
+    iIntros "{$ξl}ξl". iMod ("Totys" with "ξl") as "[tys $]". iModIntro.
+    iExists _. by iFrame.
+  Qed.
+  Next Obligation.
+    iIntros (????[|?]) "*%*% LFT In In' token κ'/="; [done|].
+    iDestruct "token" as (?->) "tys". iIntros "!>!>!>".
+    iMod (ty_shr_proph_big_sepM with "LFT In In' tys κ'") as "Toκ'"; [done|done|].
+    iIntros "!>!>". iApply (step_fupdN_wand with "Toκ'").
+    iIntros ">(%&%&%& ξl & Toκ') !>". iExists _, _. iSplit; [done|].
+    iIntros "{$ξl}ξl". by iMod ("Toκ'" with "ξl") as "$".
+  Qed.
+
+  Global Instance vec_ty_ne {𝔄} : NonExpansive (@ghostptrtoken_ty 𝔄).
+  Proof.
+    constructor.
+    exact.  
+    unfold ty_lfts. unfold ghostptrtoken_ty. eapply ty_lfts_ne. exact. 
+    unfold ty_E. unfold ghostptrtoken_ty. eapply ty_E_ne. exact.
+    unfold ty_own. unfold ghostptrtoken_ty.
+    assert (ty_size x = ty_size y). eapply ty_size_ne. exact.
+    rewrite H0.
+    intros ????. do 13 f_equiv. apply ty_own_ne; [done|done|done|done|done].
+    unfold ty_shr. unfold ghostptrtoken_ty.
+    intros ?????. do 9 f_equiv.
+    apply ty_shr_ne; [done|done|done|done|done|done].
+  Qed.
+End token.
